\documentclass[12pt]{article}
\usepackage{amsmath}
\usepackage{amsfonts}
\usepackage{parskip}
\usepackage{amsthm}
\usepackage{thmtools}
\usepackage[headheight=15pt]{geometry}
\geometry{a4paper, left=20mm, right=20mm, top=30mm, bottom=30mm}
\usepackage{graphicx}
\usepackage{bm} % for bold font in math mode - command is \bm{text}
\usepackage{enumitem}
\usepackage{fancyhdr}
\usepackage{amssymb} % for stacked arrows and other shit
\pagestyle{fancy}
\usepackage{changepage}
\usepackage{mathcomp}
\usepackage{tcolorbox}

\declaretheoremstyle[headfont=\normalfont]{normal}
\declaretheorem[style=normal]{Theorem}
\declaretheorem[style=normal]{Proposition}
\declaretheorem[style=normal]{Lemma}
\newcounter{ProofCounter}
\newcounter{ClaimCounter}[ProofCounter]
\newcounter{SubClaimCounter}[ClaimCounter]
\newenvironment{Proof}{\stepcounter{ProofCounter}\textsc{Proof.}}{\hfill$\square$}
\newenvironment{claim}[1]{\vspace{1mm}\stepcounter{ClaimCounter}\par\noindent\underline{\bf Claim \theClaimCounter:}\space#1}{}
\newenvironment{claimproof}[1]{\par\noindent\underline{Proof of claim \theClaimCounter:}\space#1}{\hfill $\blacksquare$ Claim \theClaimCounter}
\newenvironment{subclaim}[1]{\stepcounter{SubClaimCounter}\par\noindent\emph{Subclaim \theClaimCounter.\theSubClaimCounter:}\space#1}{}
% \newenvironment{subclaimproof}[1]{\begin{adjustwidth}{2em}{0pt}\par\noindent\emph{Proof of subclaim \theClaimCounter.\theSubClaimCounter:}\space#1}{\hfill
% $\blacksquare$ \emph{Subclaim \theClaimCounter.\theSubClaimCounter}\vspace{5mm}\end{adjustwidth}}
\newenvironment{subclaimproof}[1]{\par\noindent\emph{Proof of subclaim \theClaimCounter.\theSubClaimCounter:}\space#1}{\hfill
$\Diamond$ \emph{Subclaim \theClaimCounter.\theSubClaimCounter}}

\title{STAT 642: HW 4}
\author{Evan P. Walsh}
\makeatletter
\let\runauthor\@author
\let\runtitle\@title
\makeatother
\lhead{\runauthor}
\chead{\runtitle}
\rhead{\thepage}
\cfoot{}



\begin{document}
% \maketitle

\def\cp{\stackrel{p}{\rightarrow}}
\def\as{\stackrel{\text{a.s.}}{\longrightarrow}}

\subsection*{1}
\begin{tcolorbox}
Suppose $X, X_{n}, Y, Y_{n}$ are random variables on a common probability space. Show that
\begin{enumerate}[label=(\alph*)]
\item if $X_{n} \stackrel{p}{\rightarrow} X$ and $X_{n}\stackrel{p}{\rightarrow}Y$, then $P(X = Y) = 1$,
\item if $X_{n}\cp X$ and $Y_{n} \cp Y$, then $X_{n} + Y_{n} \cp X + Y$,
\item if $X_{n}\cp X$ and $Y_{n}\cp Y$, then $X_{n}Y_{n}\cp XY$, 
\item and if $X_{n}\cp X$, $Y_{n}\cp Y$ and $g$ is a continuous function on $\mathbb{R}^{2}$, then $g(X_{n},Y_{n})\cp g(X,Y)$.
\end{enumerate}
\end{tcolorbox}
\begin{enumerate}[label=(\alph*)]
\item \begin{Proof}
We need to show that $P(X - y = 0) = 1$, or $P(|X - Y| > 0) = 0$, or $P(|X - Y| > \epsilon) = 0$ for all $\epsilon > 0$. But, since $|X - Y| \leq |X -
X_{n}| + |X_{n} - Y|$,
\[ P(|X - Y| > \epsilon) \leq P(|X - X_{n}| + |X_{n} - Y| > \epsilon) \leq P(|X - X_{n}| > \epsilon/2) + P(|X_{n} - Y| > \epsilon/2).\]
But the right-hand side of the above inequality goes to 0 as $n\rightarrow \infty$, independent of $\epsilon$. Hence $P(|X-Y| > 0) = 0$.
\end{Proof}

\item \begin{Proof} Let $\epsilon > 0$. Since $|(X_{n} + Y_{n}) - (X+Y)| \leq |X_{n} - X| + |Y_{n} - Y|$,
\[ P(|(X_{n} + Y_{n}) - (X + Y) > \epsilon) \leq P(|X_{n} - X| + |Y_{n} - Y| > \epsilon) \leq P(|X_{n} - X|>\epsilon/2) + P(|Y_{n}-Y| > \epsilon/2).
\]
But the right-hand side of the above inequality goes to 0 as $n\rightarrow\infty$. Hence $X_{n} + Y_{n}\cp X + Y$.
\end{Proof}

\item \begin{Proof}
Let $\epsilon > 0$. Since 
\[ |X_{n}Y_{n} - XY| = |X_{n}Y_{n} - XY + X_{n}Y - X_{n}Y| \leq |X_{n}|\cdot |Y_{n} - Y| + |Y|\cdot |X_{n} - X|, \]
\begin{align*}
P(|X_{n}Y_{n} - XY| > \epsilon) & \leq P(|X_{n}|\cdot |Y_{n} - Y| + |Y|\cdot |X_{n} - X| > \epsilon \\
& \leq P(|X_{n}|\cdot |Y_{n}-Y| > \epsilon/2) + P(|Y|\cdot |X_{n} - X| > \epsilon/2) \\
& = P(\left\{ |X_{n}|\cdot |Y_{n}-Y| > \epsilon/2 \right\}\cap \left\{ |X_{n}-X|\leq 1 \right\}) \\
& \qquad + P(\left\{ |X_{n}|\cdot |X_{n}-Y| > \epsilon/2 \right\} 
\cap\left\{ |X_{n}-X|>1 \right\}) \\
& \qquad + P(|Y|\cdot |X_{n} -X| > \epsilon/2) \\
& = P([|X| + 1]|Y_{n} - Y| > \epsilon/2)  \rightarrow 0\\
& \qquad + P(|X_{n} - X| > 1) \rightarrow 0\\
& \qquad + P(|Y|\cdot |X_{n} - X| > \epsilon/2) \rightarrow 0
\end{align*}
Since everything on the right-hand side goes to 0 as $n\rightarrow\infty$, $X_{n}Y_{n}\cp XY$.
\end{Proof}

\item \begin{Proof}
Let $\epsilon > 0$. Since $g$ is continuous, there exists $\delta > 0$ such that $|X_{n} - X| + |Y_{n} - Y| \leq \delta$ implies $|g(X_{n},Y_{n}) -
g(X,Y)| \leq \epsilon$. Thus,
\begin{align*}
P(|g(X_{n},Y_{n}) - g(X,Y)| > \epsilon) & \leq P(|X_{n} - X| + |Y_{n} - Y| > \delta) \\
& \leq P(|X_{n} - X| > \delta/2) + P(|Y_{n} - Y|>\delta/2).
\end{align*}
But everything on the right-hand side goes to 0 as $n\rightarrow\infty$. Therefore $g(X_{n},Y_{n}) \cp g(X,Y)$. 
\end{Proof}
\end{enumerate}

\subsection*{2}
\begin{tcolorbox}
Show that if $\left\{ X_{n} \right\}_{n=0}^{\infty}$ is a sequence of independent random variables and $X_{n} \cp X$, then $X$ is degenerate.
\end{tcolorbox}
\begin{Proof}

\end{Proof}

\subsection*{3}
\begin{tcolorbox}
For any sequence $\left\{ X_{n} \right\}_{n=0}^{\infty}$ of random variables with $X_{n}\cp X$, show that 
\[ P(\liminf_{n\rightarrow\infty}X_{n}\leq X\leq \limsup_{n\rightarrow\infty}X_{n}) = 1. \]
\end{tcolorbox}

\subsection*{4}
\begin{tcolorbox}
Let $X, X_{0}, X_{1}, \hdots$ be random variables and suppose that for some $r > 0$,
\[ E|X_{n} - X|^{r} \rightarrow 0 \ \text{ as } \ n \rightarrow \infty. \]
Prove that $X_{n}\cp X$.
\end{tcolorbox}

\subsection*{5}
\begin{tcolorbox}
Let $X, X_{0}, X_{1}, \hdots$ be random variables and suppose that for some $r > 0$,
\[ \sum_{n=0}^{\infty}E|X_{n} - X|^{r} < \infty. \]
Prove that $X_{n} \as X$.
\end{tcolorbox}

\subsection*{6}
\begin{tcolorbox}
Suppose $X_{1}, X_{2}, \hdots$ are random variables. For each $n \geq 1$, let $S_{n} := \sum_{j=1}^{n}X_{j}$. Let $b_{1}, b_{2}, \hdots \in
\mathbb{R}$ such that $0 < b_{n} < \infty$ and $b_{n} = \mathcal{0}(b_{n+1})$ for all $n \geq 1$. Prove that if 
$\frac{S_{n}}{b_{n}} \as 0$, then $\frac{X_{n}}{b_{n}} \as 0$.
\end{tcolorbox}

\end{document}

