\documentclass[12pt]{article}
\usepackage{amsmath}
\usepackage{amsfonts}
\usepackage{parskip}
\usepackage{amsthm}
\usepackage{thmtools}
\usepackage[headheight=15pt]{geometry}
\geometry{a4paper, left=20mm, right=20mm, top=30mm, bottom=30mm}
\usepackage{graphicx}
\usepackage{bm} % for bold font in math mode - command is \bm{text}
\usepackage{enumitem}
\usepackage{fancyhdr}
\usepackage{amssymb} % for stacked arrows and other shit
\pagestyle{fancy}
\usepackage{changepage}
\usepackage{mathcomp}
\usepackage{tcolorbox}

\declaretheoremstyle[headfont=\normalfont]{normal}
\declaretheorem[style=normal]{Theorem}
\declaretheorem[style=normal]{Proposition}
\declaretheorem[style=normal]{Lemma}
\newcounter{ProofCounter}
\newcounter{ClaimCounter}[ProofCounter]
\newcounter{SubClaimCounter}[ClaimCounter]
\newenvironment{Proof}{\stepcounter{ProofCounter}\textsc{Proof.}}{\hfill$\square$}
\newenvironment{Solution}{\stepcounter{ProofCounter}\textbf{Solution:}}{\hfill$\square$}
\newenvironment{claim}[1]{\vspace{1mm}\stepcounter{ClaimCounter}\par\noindent\underline{\bf Claim \theClaimCounter:}\space#1}{}
\newenvironment{claimproof}[1]{\par\noindent\underline{Proof of claim \theClaimCounter:}\space#1}{\hfill $\blacksquare$ Claim \theClaimCounter}
\newenvironment{subclaim}[1]{\stepcounter{SubClaimCounter}\par\noindent\emph{Subclaim \theClaimCounter.\theSubClaimCounter:}\space#1}{}
% \newenvironment{subclaimproof}[1]{\begin{adjustwidth}{2em}{0pt}\par\noindent\emph{Proof of subclaim \theClaimCounter.\theSubClaimCounter:}\space#1}{\hfill
% $\blacksquare$ \emph{Subclaim \theClaimCounter.\theSubClaimCounter}\vspace{5mm}\end{adjustwidth}}
\newenvironment{subclaimproof}[1]{\par\noindent\emph{Proof of subclaim \theClaimCounter.\theSubClaimCounter:}\space#1}{\hfill
$\Diamond$ \emph{Subclaim \theClaimCounter.\theSubClaimCounter}}

\allowdisplaybreaks{}

% chktex-file 3

\title{STAT 520: Assignment 6}
\author{Evan P. Walsh}
\makeatletter
\makeatother
\lhead{Evan P. Walsh}
\chead{STAT 520: Assignment 6}
\rhead{\thepage}
\cfoot{}

\begin{document}
\maketitle

\subsection*{1} (a) The posterior $p(\beta|\bm{y})$ can be derived as follows:
\begin{align*}
  p(\beta|\bm{y}) & \propto f(\bm{y}|\beta)\pi(\beta|\mu_{\beta}, \tau_{\beta}^{2}) \\
  & = (2\pi \sigma^{2})^{-n/2}\exp\left\{ -\frac{1}{2\sigma^{2}}\sum_{i=1}^{n}(y_i - \beta x_i)^{2} \right\}(2\pi \tau_{\beta}^{2})^{-1/2}\exp\left\{
  -\frac{1}{2\tau_{\beta}^{2}}(\beta - \mu_{\beta})^{2} \right\} \\
  & \propto\exp\left\{ -\frac{1}{2\sigma^{2}}\left[ \sum_{i=1}^{n}y_i^2 - 2\beta\sum_{i=1}^{n}x_i y_i + \beta^{2}\sum_{i=1}^{n}x_i^2 \right] - 
  \frac{1}{2\tau_{\beta}^{2}}\left[ \beta^{2} - 2\beta \mu_{\beta} + \mu_{\beta}^{2} \right]\right\} \\
  & = \exp\left\{ -\frac{1}{2\sigma^{2}\tau_{\beta}^{2}}\left[ \tau_{\beta}^{2}\sum_{i=1}^{n}y_i^2 - 2\tau_{\beta}^2\beta \sum_{i=1}^{n}x_i y_i + 
    \tau_{\beta}^2\beta^2\sum_{i=1}^{n}x_i^2 + \sigma^2\beta^2 - 2\sigma^2\beta\mu_{\beta} + \sigma^2\mu_{\beta}^2\right] \right\} \\
    & = \exp\left\{ -\frac{\tau_{\beta}^{2}\sum_{i=1}^{n}x_i^2 + \sigma^{2}}{2\sigma^{2}\tau_{\beta}^{2}}\left[ \beta^{2} - 
    2\left( \frac{\tau_{\beta}^2\sum_{i=1}^{n}x_i y_i + \sigma^{2}\mu_{\beta}}{\tau_{\beta}^2\sum_{i=1}^{n}x_i^2 + \sigma^2} \right)\beta + 
\frac{\tau_{\beta}^2\sigma^2\mu_{\beta}^2\sum_{i=1}^n y_i^2}{\tau_{\beta}^2\sum_{i=1}^{n}x_i^2 + \sigma^2}\right] \right\} \\
    & \propto \exp\left\{ -\frac{\tau_{\beta}^{2}\sum_{i=1}^{n}x_i^2 + \sigma^{2}}{2\sigma^{2}\tau_{\beta}^{2}}\left[ \left(\beta - 
    \frac{\tau_{\beta}^2\sum_{i=1}^{n}x_i y_i + \sigma^{2}\mu_{\beta}}{\tau_{\beta}^2\sum_{i=1}^{n}x_i^2 + \sigma^2} \right)^{2}\right] \right\},
\end{align*}
which is the kernal of a normal distribution with mean 
\begin{equation}
  \frac{\tau_{\beta}^2\sum_{i=1}^{n}x_i y_i + \sigma^{2}\mu_{\beta}}{\tau_{\beta}^2\sum_{i=1}^{n}x_i^2 + \sigma^2}
  \label{1.1}
\end{equation}
and variance
\begin{equation}
  \left(\frac{\tau_{\beta}^{2}\sum_{i=1}^{n}x_i^2 + \sigma^{2}}{\sigma^{2}\tau_{\beta}^{2}}\right)^{-1}.
  \label{1.2}
\end{equation}

(b) 

\end{document}

